{
  "cells": [
    {
      "cell_type": "markdown",
      "metadata": {
        "id": "55J0JCNo4heY"
      },
      "source": [
        "1. Find the value of T(2) for the recurrence relation T(n) = 3T(n-1) + 12n, given that T(0)=5.\n",
        "\n",
        "sol:-\n",
        "\n",
        "                T(n) = 3T(n-1) + 12n\n",
        "                n=2, T(0)=5\n",
        "\n",
        "                =>T(2) = 3T(2-1) + 122\n",
        "                => T(2) = 3T(1) + 122\n",
        "                => T(2) = 3[3T(1-1)+121] + 24\n",
        "                => T(2) = 3[3T(0)+121] + 24\n",
        "                => T(2) = 3[35+121] + 24\n",
        "                => T(2) = 3[15+12] + 24\n",
        "                => T(2) = 3*27 + 24\n",
        "                => T(2) = 81 + 24\n",
        "                => T(2) = 105\n",
        "\n",
        "\n",
        "\n",
        "2. Given a recurrence relation, solve it using the substitution method:\n",
        "\n",
        "a. T(n) = T(n-1) + c\n",
        "\n",
        "sol:-\n",
        "\n",
        "                    let, T(1) = b\n",
        "                    T(n) = T(n-1) + c   ----------(1)\n",
        "                    =>T(n-1) = T(n-1-1) + c\n",
        "                    =>T(n-1) = T(n-2) + c   --------(2)\n",
        "\n",
        "                    by substitute the value of 2 in 1 ,\n",
        "                    =>T(n) = T(n-2) + 2c\n",
        "                    Then,\n",
        "                    =>T(n) = T(n-3) + 3c\n",
        "\n",
        "                    After k times,\n",
        "                    T(n) = T(n-k) + k*c\n",
        "                    if n-k=1, k=(n-1)\n",
        "                    then,\n",
        "                    T(n) = T(n-n+1) + (n-1)c\n",
        "                    T(n) = T(1) + (n-1)c\n",
        "                    T(n) = b + (n-1)c\n",
        "                 \n",
        "                  ------------O(n)\n",
        "\n",
        "\n",
        "\n",
        "b. T(n) = 2T(n/2) + n\n",
        "\n",
        "sol:-\n",
        "\n",
        "                    let, T(1) = b\n",
        "                    T(n) = 2T(n/2) + n   ----------(1)\n",
        "                    =>T(n/2) = 2T(n/4) + n/2  -------(2)\n",
        "\n",
        "                    by substitute the value of 2 in 1 ,\n",
        "                    =>T(n) = 4T(n/4) + 2n\n",
        "                    Then,\n",
        "                    =>T(n) = 2^3[T(n/2^3)] + 3n\n",
        "\n",
        "                    After k times,\n",
        "                    T(n) = 2^k[T(n/2^k)] + k*n\n",
        "\n",
        "                    if n/2^k=1, n=2^k\n",
        "                    log(n) = klog2\n",
        "                    k = log(n)\n",
        "                    then,\n",
        "                    T(n) = nT(1) + nlog(n)\n",
        "                    T(n) = nb + nlog(n)\n",
        "\n",
        "                ---------------O(nlogn)\n",
        "\n",
        "\n",
        "c. T(n) = 2T(n/2) + c\n",
        "\n",
        "sol:-\n",
        "\n",
        "                    let, T(1) = b\n",
        "                    T(n) = 2T(n/2) + c   ----------(1)\n",
        "                    =>T(n/2) = 2T(n/4) + c  -------(2)\n",
        "\n",
        "                    by substitute the value of 2 in 1 ,\n",
        "                    =>T(n) = 4T(n/4) + 2c\n",
        "                    Then,\n",
        "                    =>T(n) = 2^3[T(n/2^3)] + 3c\n",
        "\n",
        "                    After k times,\n",
        "                    T(n) = 2^k[T(n/2^k)] + k.c\n",
        "\n",
        "                    if n/2^k=1, n=2^k\n",
        "                    log(n) = klog2,\n",
        "                    k = log(n)\n",
        "                    then,\n",
        "                    T(n) = nT(1) + log(n).c\n",
        "                    T(n) = nb + log(n).c\n",
        "                    \n",
        "                    -------------O(log(n))\n",
        "\n",
        "\n",
        "d. T(n) = T(n/2) + c\n",
        "\n",
        "sol:-\n",
        "\n",
        "                    let, T(1) = b\n",
        "                    T(n) = T(n/2) + c   ----------(1)\n",
        "                    =>T(n/2) = T(n/4) + c  -------(2)\n",
        "\n",
        "                    by substitute the value of 2 in 1 ,\n",
        "                    =>T(n) = T(n/4) + 2c\n",
        "                    Then,\n",
        "                    =>T(n) = [T(n/2^3)] + 3c\n",
        "\n",
        "                    After k times,\n",
        "                    T(n) = [T(n/2^k)] + k.c\n",
        "\n",
        "                    if n/2^k=1, n=2^k\n",
        "                    log(n) = klog2,\n",
        "                    k = log(n)\n",
        "                    then,\n",
        "                    T(n) = T(1) + log(n).c\n",
        "                    T(n) = b + log(n).c\n",
        "\n",
        "                    ---------O(logn)\n",
        "\n",
        "3. Given a recurrence relation, solve it using the recursive tree approach:\n",
        "\n",
        "a. T(n) = 2T(n-1) +1\n",
        "\n",
        "                    by recursive tree we get to know,\n",
        "\n",
        "                    2^0 + 2^1 + 2^2 + 2^3 + ------------ +2^k = S\n",
        "                    it's GP series,\n",
        "                    so,  sum of GP series Sn = a(r^n -1)/(r – 1), if r > 1\n",
        "                    here, a=1, r=2, n=k\n",
        "                            Sn = 1(2^n-1)/(2– 1)\n",
        "                            = 2^n -1\n",
        "                          \n",
        "                     So,T(n) = 2T(n-1) +1-----------> O(2^n)\n",
        "\n",
        "b. T(n) = 2T(n/2) + n\n",
        "                    \n",
        "                    by recursive tree we get to know,\n",
        "                       \n",
        "                       T(n) = 2T(n/2) + n -------------> nk\n",
        "\n",
        "                    \n",
        "                    Assume, n/2^k = 1,\n",
        "                            n = 2^k\n",
        "                            log(n)=klog2\n",
        "                            k=log(n)\n",
        "\n",
        "                        nk = n.log(n)\n",
        "\n",
        "                    So, T(n) = 2T(n/2) + n ---------->  O(nlog(n))\n"
      ]
    },
    {
      "cell_type": "code",
      "execution_count": 11,
      "metadata": {},
      "outputs": [
        {
          "name": "stdout",
          "output_type": "stream",
          "text": [
            "not a pallendrom\n"
          ]
        }
      ],
      "source": []
    }
  ],
  "metadata": {
    "colab": {
      "provenance": []
    },
    "kernelspec": {
      "display_name": "Python 3",
      "name": "python3"
    },
    "language_info": {
      "codemirror_mode": {
        "name": "ipython",
        "version": 3
      },
      "file_extension": ".py",
      "mimetype": "text/x-python",
      "name": "python",
      "nbconvert_exporter": "python",
      "pygments_lexer": "ipython3",
      "version": "3.12.2"
    }
  },
  "nbformat": 4,
  "nbformat_minor": 0
}
